new indexing approach

secure_api/box/functor_box/Box.ODH.fsti
@@ -7,12 +7,14 @@ open FStar.HyperStack.ST
 
 open Box.Key
 
-module ID = Box.Indexing
+module ID = Box.Index
 
 val dh_share: eqtype
 val dh_exponent: eqtype
 
 val smaller: i1:dh_share -> i2:dh_share -> b:bool{b ==> i1 <> i2}
+
+let key_id = i:(dh_share * dh_share){b2t (smaller (fst i) (snd i))}
 
 val total_order_lemma: (i1:dh_share -> i2:dh_share -> Lemma
   (requires True)
@@ -22,11 +24,12 @@ val total_order_lemma: (i1:dh_share -> i2:dh_share -> Lemma
 
 val share_from_exponent: dh_exponent -> Tot dh_share
 
-type index_module = im:ID.index_module{ID.get_subId im == dh_share}
+type index_module = im:ID.index_module{ID.id im == dh_share}
+type key_index_module = im:ID.index_module{ID.id im == key_id}
 
-val odh_module: im:index_module -> key_module im -> Type0
+val odh_module: im:index_module -> kim:key_index_module -> key_module kim -> Type0
 
-val create: im:index_module -> km:key_module im -> rgn:log_region im -> odh_module im km
+val create: im:index_module -> kim:key_index_module -> km:key_module kim -> rgn:log_region im -> odh_module im kim km
 
 (**
   A DH public key containing its raw byte representation. All ids of DH keys have to be unfresh and registered (e.g. marked as either honest
@@ -48,7 +51,7 @@ val compatible_keys: sk:skey -> pk:pkey -> t:Type0{t <==> pk =!= get_pkey sk}
 (**
   A helper function to obtain the raw bytes of a DH public key.
 *)
-val pk_get_share: pk:pkey -> Tot (dh_sh:dh_share) //{dh_sh = pk.pk_share})
+val pk_get_share: pk:pkey -> Tot (dh_sh:dh_share) //{dh_sh = pk.pk_sharite numbersre})
 
 val lemma_pk_get_share_inj: pk:pkey -> Lemma
   (requires True)
@@ -63,45 +66,50 @@ A helper function to obtain the share that corresponds to a DH secret key.
 *)
 val sk_get_share: sk:skey -> Tot (dh_sh:dh_share{dh_sh = share_from_exponent (get_skeyGT sk)})
 
-val leak_skey: im:index_module -> sk:skey{ID.dishonest im (ID.SUBID (sk_get_share sk))} -> Tot (raw:dh_exponent{raw=get_skeyGT sk})
+val leak_skey: im:index_module -> sk:skey{ID.dishonest im (sk_get_share sk)} -> Tot (raw:dh_exponent{raw=get_skeyGT sk})
 
 val keygen: unit -> ST (dh_pair:(pkey * skey){fst dh_pair == get_pkey (snd dh_pair)})
   (requires (fun h0 -> True))
   (ensures (fun h0 _ h1 -> modifies_none h0 h1))
 
-val coerce_pkey: im:index_module -> dh_sh:dh_share{ID.dishonest im (ID.SUBID dh_sh)} -> Tot (pk:pkey{pk_get_share pk=dh_sh})
+val coerce_pkey: im:index_module -> dh_sh:dh_share{ID.dishonest im dh_sh} -> Tot (pk:pkey{pk_get_share pk=dh_sh})
 
 (**
   coerce_keypair allows the adversary to coerce a DH exponent into a DH private key. The corresponding DH public key
   is generated along with it. Both keys are considered dishonest and the id is considered unfresh after coercion.
 *)
-val coerce_keypair: im:index_module -> dh_exp:dh_exponent{ID.dishonest im (ID.SUBID (share_from_exponent dh_exp))} -> Tot (dh_pair:(k:pkey{pk_get_share k = share_from_exponent dh_exp}) * (k:skey{get_skeyGT k=dh_exp}))
+val coerce_keypair: im:index_module -> dh_exp:dh_exponent{ID.dishonest im (share_from_exponent dh_exp)} -> Tot (dh_pair:(k:pkey{pk_get_share k = share_from_exponent dh_exp}) * (k:skey{get_skeyGT k=dh_exp}))
 
+
+val compose_ids: s1:dh_share -> s2:dh_share{s2 <> s1} -> (i:(dh_share * dh_share){b2t (smaller (fst i) (snd i))})
 
 (**
   GTot specification of the prf_odh function for use in type refinements.
 *)
-val prf_odhGT: im:index_module -> sk:skey -> pk:pkey{compatible_keys sk pk} -> GTot aes_key
+val prf_odhGT: sk:skey -> pk:pkey{compatible_keys sk pk} -> GTot aes_key
 
 val lemma_shares: sk:skey -> Lemma
   (requires True)
   (ensures (pk_get_share (get_pkey sk)) == sk_get_share sk)
   [ SMTPat (sk_get_share sk)]
 
-val prf_odh: im:index_module -> km:key_module im -> om:odh_module im km  -> sk:skey -> pk:pkey{compatible_keys sk pk} -> ST (k:Key.get_keytype im km{Key.get_index im km k = (ID.compose_ids im (pk_get_share pk) (sk_get_share sk))} )
+
+
+val prf_odh: im:index_module -> kim:key_index_module -> km:key_module kim -> om:odh_module im kim km  -> sk:skey -> pk:pkey{compatible_keys sk pk} -> ST (k:Key.get_keytype kim km{Key.get_index kim km k = (compose_ids (pk_get_share pk) (sk_get_share sk))} )
   (requires (fun h0 ->
-    let i = ID.compose_ids im (pk_get_share pk) (sk_get_share sk) in
-    ID.registered im (ID.ID i)
-    /\ Key.invariant im km h0
+    let i = compose_ids (pk_get_share pk) (sk_get_share sk) in
+    ID.registered kim i
+    /\ Key.invariant kim km h0
   ))
   (ensures (fun h0 k h1 ->
-    let i = ID.compose_ids im (pk_get_share pk) (sk_get_share sk) in
-    (ID.honest im (ID.ID i) ==> modifies (Set.singleton (Key.get_log_region im km)) h0 h1)
+    let i = compose_ids (pk_get_share pk) (sk_get_share sk) in
+    (ID.honest kim i ==> modifies (Set.singleton (Key.get_log_region kim km)) h0 h1)
     // We should guarantee, that the key is randomly generated. Generally, calls to prf_odh should be idempotent. How to specify that?
     // Should we have a genPost condition that we guarantee here?
-    /\ (ID.dishonest im (ID.ID i) ==>
-                        (Key.leak im km k = prf_odhGT im sk pk // Functional correctness. Spec should be external in Spec.Cryptobox.
+    /\ (ID.dishonest kim i ==>
+                        (Key.leak kim km k = prf_odhGT sk pk // Functional correctness. Spec should be external in Spec.Cryptobox.
                         /\ h0 == h1))
-    /\ (modifies (Set.singleton (Key.get_log_region im km)) h0 h1 \/ h0 == h1)
-    /\ Key.invariant im km h1
+    /\ (modifies (Set.singleton (Key.get_log_region kim km)) h0 h1 \/ h0 == h1)
+    /\ Key.invariant kim km h1
   ))
+ 
